src/Init/Prelude.lean
@@ -2920,31 +2920,31 @@ protected def List.hasDecEq {α : Type u} [DecidableEq α] : (a b : List α) →
       | isFalse nabs => isFalse (fun h => List.noConfusion h (fun _ habs => absurd habs nabs))
     | isFalse nab => isFalse (fun h => List.noConfusion h (fun hab _ => absurd hab nab))
 
-/--
-Expands the first match step to allow decidable equality of empty lists while
-keeping the overlapping solutions equivalent.
--/
 instance {α : Type u} [DecidableEq α] : DecidableEq (List α) := fun xs ys =>
+  /-
+  The first match step is expanded to make this instance
+  maximally-definitionally-equivalent to the compare-with-empty-list cases.
+  -/
   match xs with
   | .nil => match ys with
     | .nil => isTrue rfl
     | .cons _ _ => isFalse List.noConfusion
   | .cons a as => match ys with
-    | .nil => isFalse (List.noConfusion ·)
+    | .nil => isFalse List.noConfusion
     | .cons b bs =>
       match decEq a b with
-      | isTrue hab  =>
+      | isTrue hab =>
         match List.hasDecEq as bs with
         | isTrue habs  => isTrue (hab ▸ habs ▸ rfl)
-        | isFalse nabs => isFalse (fun h => List.noConfusion h (fun _ habs => absurd habs nabs))
-      | isFalse nab => isFalse (fun h => List.noConfusion h (fun hab _ => absurd hab nab))
+        | isFalse nabs => isFalse (List.noConfusion · (fun _ habs => absurd habs nabs))
+      | isFalse nab => isFalse (List.noConfusion · (fun hab _ => absurd hab nab))
 
-instance instDecidableNilEq (a : List α) : Decidable (Eq List.nil a) :=
+instance List.instDecidableNilEq (a : List α) : Decidable (Eq List.nil a) :=
   match a with
   | .nil => isTrue rfl
   | .cons _ _ => isFalse List.noConfusion
 
-instance instDecidableEqNil (a : List α) : Decidable (Eq a List.nil) :=
+instance List.instDecidableEqNil (a : List α) : Decidable (Eq a List.nil) :=
   match a with
   | .nil => isTrue rfl
   | .cons _ _ => isFalse List.noConfusion
