tests/lean/run/arrayDecEq.lean
@@ -10,12 +10,14 @@ def listR (a : Array α) := if #[] = a then 1 else 2
 /-- info: 2 -/
 #guard_msgs in #eval listL #[()]
 
+
+-- test instance diamonds
+example :
+    @Array.instDecidableEmpEq α #[] = @Array.instDecidableEqEmp α #[] := by
+  with_reducible_and_instances rfl
+
 section
 variable {α : Type u} [DecidableEq α]
-
--- test for instance diamonds
-
-/-
 example (x : Array α) :
     Array.instDecidableEq x #[] = Array.instDecidableEqEmp x := by
   with_reducible_and_instances rfl
@@ -24,4 +26,3 @@ example (x : Array α) :
     Array.instDecidableEq #[] x = Array.instDecidableEmpEq x := by
   with_reducible_and_instances rfl
 end
--/
